Matcher invariant is actually not used; remove it from the proofs
Actually, we already prove what we need (i.e. the match state advances in direction dir for any Matcher compiled with direction dir) in our proofs, albeit not very obviously

WarblreEquiv/FunctTreeCompute/EquivDef.v
@@ -39,12 +39,11 @@ Section EquivDef.
   performs the actions described in act in the direction dir when: *)
   Definition equiv_cont (mc: MatcherContinuation) (gl: open_groups) (forbgroups: list group_id) (act: actions) (dir: Direction) (str0: string) (rer: RegExpRecord): Prop :=
     forall (gm: group_map) (ms: MatchState) (inp: input) (res: option MatchState) (fuel: nat) (t: tree),
-      (* for all corresponding tuples of a valid MatchState ms, an input inp, a group map gm 
+      (* for all corresponding tuples of a MatchState ms, an input inp, a group map gm 
       and a list of open groups gl that use the input string str0, *)
       input_compat inp str0 ->
       equiv_groupmap_ms gm ms -> group_map_equiv_open_groups gm gl ->
       ms_matches_inp ms inp ->
-      MatchState.Valid (MatchState.input ms) rer ms ->
       (* such that ms is valid with respect to the checks in act *)
       ms_valid_wrt_checks ms act dir ->
       (* and gm does not define any of the groups in the forbidden groups, *)
